theories/Control.v
@@ -173,18 +173,6 @@ Definition join
   : m a :=
   x >>= id.
 
-(** * Monad Transformer
-
- *)
-
-Class MonadTrans
-      (t: forall (m: Type -> Type) `{Monad m}, Type -> Type)
-  := { monad_trans_is_monad (m: Type -> Type) `{Monad m} :> Monad (t m)
-     ; lift (m: Type -> Type) `{Monad m} (a: Type): m a -> t m a
-     }.
-
-Arguments lift [t _ m _ a] (_).
-
 Notation "a <- p ; q" :=
   (bind p (fun a => q)) (at level 99, right associativity, p at next level)
   : free_control_scope.
