theories/Control/Classes.v
@@ -1,0 +1,29 @@
+Require Import FreeSpec.Control.
+Require Import FreeSpec.WEq.
+
+(** Monad Transformer
+
+ *)
+
+Class MonadTrans
+      (t: forall (m: Type -> Type) `{Monad m}, Type -> Type)
+  := { monad_trans_is_monad (m: Type -> Type) `{Monad m} :> Monad (t m)
+     ; lift (m: Type -> Type) `{Monad m} (a: Type): m a -> t m a
+     }.
+
+Arguments lift [t _ m _ a] (_).
+
+(** * State Monad
+
+ *)
+
+Class MonadState
+      (m: Type -> Type)
+      (s: Type) :=
+  { monadstate_is_monad :> Monad m
+  ; put: s -> m unit
+  ; get: m s
+  }.
+
+Arguments put [m s _] (_).
+Arguments get [m s _].
